ballet/63/Src/Eiffel/interface/new_graphical/windows/development_window/initialization/eb_development_window_main_builder.e
@@ -155,6 +155,7 @@ feature -- Command
 			l_restore_editors_command: EB_RESTORE_EDITORS_COMMAND
 
 			l_verify_class_command: EB_VERIFY_CLASS_COMMAND
+			l_verify_cluster_command: EB_VERIFY_CLUSTER_COMMAND
 
 			l_editor_font_zoom_in_command: EB_EDITOR_FONT_ZOOM_IN_COMMAND
 			l_editor_font_zoom_in_numpad_command: ES_EDITOR_FONT_ZOOM_IN_NUMPAD_COMMAND
@@ -383,6 +384,8 @@ feature -- Command
 				-- Ballet commands
 			create l_verify_class_command.make (develop_window)
 			develop_window.commands.set_verify_class_command (l_verify_class_command)
+			create l_verify_cluster_command.make (develop_window)
+			develop_window.commands.set_verify_cluster_command (l_verify_cluster_command)
 
 
 				-- Add history commands to toolbarable_commands.
