ballet/63/Src/eve_proofs/ep_default_names.e
@@ -1,0 +1,115 @@
+indexing
+	description:
+		"[
+			Generator for default names
+		]"
+	date: "$Date$"
+	revision: "$Revision$"
+
+class EP_DEFAULT_NAMES
+
+feature -- Access
+
+	attribute_name (a_feature: !FEATURE_I): STRING
+			-- Name of attribute `a_feature' as used in Boogie code
+		require
+			is_attribute: a_feature.is_attribute
+		local
+			l_class_name: STRING
+		do
+			l_class_name := a_feature.written_class.name_in_upper
+			Result := "field." + l_class_name + "." + mangled_feature_name (a_feature)
+		end
+
+	functional_feature_name (a_feature: !FEATURE_I): STRING
+			-- Functional name of `a_feature' as used in Boogie code
+		local
+			l_class_name: STRING
+		do
+			l_class_name := a_feature.written_class.name_in_upper
+			Result := "fun." + l_class_name + "." + mangled_feature_name (a_feature)
+		end
+
+	procedural_feature_name (a_feature: !FEATURE_I): STRING
+			-- Procedural name of `a_feature' as used in Boogie code
+		local
+			l_class_name: STRING
+		do
+			l_class_name := a_feature.written_class.name_in_upper
+			Result := "proc." + l_class_name + "." + mangled_feature_name (a_feature)
+		end
+
+	creation_routine_name (a_feature: !FEATURE_I): STRING
+			-- Name of creation routine `a_feature' as used in Boogie code
+		local
+			l_class_name: STRING
+		do
+			l_class_name := a_feature.written_class.name_in_upper
+			Result := "create." + l_class_name + "." + mangled_feature_name (a_feature)
+		end
+
+	argument_name (a_name: STRING): STRING
+			-- Name of an argument as used in Boogie code
+		do
+			Result := "arg." + a_name
+		end
+
+feature {NONE} -- Implementation
+
+	mangled_feature_name (a_feature: !FEATURE_I): STRING
+			-- Mangled feature name of `a_feature'
+		local
+			l_name: STRING
+		do
+			l_name := a_feature.feature_name
+			if a_feature.is_infix then
+				Result := mangled_operator_name (l_name.substring (8, l_name.count-1))
+			elseif a_feature.is_prefix then
+				Result := mangled_operator_name (l_name.substring (9, l_name.count-1))
+			else
+				Result := l_name
+			end
+		end
+
+	mangled_operator_name (a_operator: STRING): STRING is
+			-- Mangled name of operator `a_operator'
+		require
+			not_empty: not a_operator.is_empty
+		do
+			if mangled_operator_names.has_key (a_operator) then
+				Result := mangled_operator_names.item (a_operator)
+			else
+					-- Free operator, create a unique name
+				Result := "op$" + mangled_operator_names.count.out
+				mangled_operator_names.put (Result, a_operator)
+			end
+		ensure
+			not_void: Result /= Void
+		end
+
+	mangled_operator_names: HASH_TABLE [STRING, STRING] is
+			-- Mangled names for default operators
+		once
+			create Result.make(19)
+			Result.compare_objects
+			Result.put ("op$not", "not")
+			Result.put ("op$plus", "+")
+			Result.put ("op$minus", "-")
+			Result.put ("op$mult", "*")
+			Result.put ("op$div", "/")
+			Result.put ("op$less", "<")
+			Result.put ("op$more", ">")
+			Result.put ("op$leq", "<=")
+			Result.put ("op$meq", ">=")
+			Result.put ("op$divdiv", "//")
+			Result.put ("op$vidvid", "\\")
+			Result.put ("op$hat", "^")
+			Result.put ("op$and", "and")
+			Result.put ("op$or", "or")
+			Result.put ("op$xor", "xor")
+			Result.put ("op$andthen", "and then")
+			Result.put ("op$orelse", "or else")
+			Result.put ("op$implies", "implies")
+		end
+
+end
