ballet/63/Src/eve_proofs/ep_environment.e
@@ -1,0 +1,55 @@
+indexing
+	description: "TODO"
+	date: "$Date$"
+	revision: "$Revision$"
+
+class EP_ENVIRONMENT
+
+inherit {NONE}
+
+	KL_SHARED_STANDARD_FILES
+		export {NONE} all end
+
+create
+	make
+
+feature{NONE} -- Initialization
+
+	make is
+			-- Initialize environment with default output stream.
+		do
+			reset
+		ensure
+			output_buffer_set: output_buffer = std.output
+		end
+
+feature -- Access
+
+	output_buffer: !KI_TEXT_OUTPUT_STREAM
+			-- Output buffer for generated Boogie code
+
+feature -- Element change
+
+	set_output_buffer (a_value: !KI_TEXT_OUTPUT_STREAM)
+			-- Set `output_buffer' to `a_value'.
+		do
+			output_buffer := a_value
+		ensure
+			output_buffer_set: output_buffer = a_value
+		end
+
+feature -- Basic operations
+
+	reset
+			-- Reset environment for new verification session.
+		do
+			if {l_buffer: KI_TEXT_OUTPUT_STREAM} std.output then
+				output_buffer := l_buffer
+			else
+				check false end
+			end
+		ensure
+			output_buffer_reset: output_buffer = std.output
+		end
+
+end
