ballet/63/Src/eve_proofs/ep_feature_list.e
@@ -1,0 +1,93 @@
+indexing
+	description:
+		"[
+			List of features which are already generated and which still need to be generated.
+		]"
+	date: "$Date$"
+	revision: "$Revision$"
+
+class EP_FEATURE_LIST
+
+create
+	make
+
+feature {NONE} -- Implementation
+
+	make
+			-- Initialize object with emtpy lists.
+		do
+				-- TODO: use more efficient data structures
+			create {LINKED_LIST [!FEATURE_I]} creation_routines_needed.make
+			create {LINKED_LIST [!FEATURE_I]} creation_routines_generated.make
+			create {LINKED_LIST [!FEATURE_I]} features_needed.make
+			create {LINKED_LIST [!FEATURE_I]} features_generated.make
+		end
+
+feature -- Access
+
+	creation_routines_needed: !LIST [!FEATURE_I]
+			-- List of creation routines which still need to be generated
+
+	creation_routines_generated: !LIST [!FEATURE_I]
+			-- List of creation routines which have already been generated
+
+	features_needed: !LIST [!FEATURE_I]
+			-- List of feature which still need to be generated
+
+	features_generated: !LIST [!FEATURE_I]
+			-- List of featurew which have already been generated
+
+feature -- Element change
+
+	record_creation_routine_needed (a_feature: !FEATURE_I)
+			-- Record that `a_feature' is needed as a creation routine.
+		do
+			if not creation_routines_generated.has (a_feature) then
+				creation_routines_needed.extend (a_feature)
+			end
+		ensure
+			not creation_routines_generated.has (a_feature) implies creation_routines_needed.has (a_feature)
+		end
+
+	record_feature_needed (a_feature: !FEATURE_I)
+			-- Record that `a_feature' is needed either in a contract or an implementation.
+		do
+			if not features_generated.has (a_feature) then
+				features_needed.extend (a_feature)
+			end
+		ensure
+			not features_generated.has (a_feature) implies features_needed.has (a_feature)
+		end
+
+feature -- Basic operations
+
+	mark_creation_routine_as_generated (a_feature: !FEATURE_I)
+			-- Mark that `a_feature' has been generated as a creation routine.
+		do
+			creation_routines_needed.prune_all (a_feature)
+			creation_routines_generated.extend (a_feature)
+		ensure
+			a_feature_not_needed: not creation_routines_needed.has (a_feature)
+			a_feature_generated: creation_routines_generated.has (a_feature)
+		end
+
+	mark_feature_generated (a_feature: !FEATURE_I)
+			-- Mark that `a_feature' has been generated as a normal feature.
+		do
+			features_needed.prune_all (a_feature)
+			features_generated.extend (a_feature)
+		ensure
+			a_feature_not_needed: not features_needed.has (a_feature)
+			a_feature_generated: features_generated.has (a_feature)
+		end
+
+	reset
+			-- Reset the lists.
+		do
+			creation_routines_needed.wipe_out
+			creation_routines_generated.wipe_out
+			features_needed.wipe_out
+			features_generated.wipe_out
+		end
+
+end
