ballet/63/Src/eve_proofs/ep_generator.e
@@ -1,0 +1,162 @@
+indexing
+	description: "TODO"
+	date: "$Date$"
+	revision: "$Revision$"
+
+class EP_GENERATOR
+
+inherit {NONE}
+
+	SHARED_EP_ENVIRONMENT
+		export {NONE} all end
+
+create
+	make
+
+feature {NONE} -- Initialization
+
+	make
+			-- Initialize generator.
+		do
+			create attribute_writer
+			create constant_writer
+			create signature_writer.make
+			create implementation_writer.make
+		end
+
+feature -- Basic operations
+
+	process_class (a_class: !CLASS_C)
+			-- Generate code for `a_class'.
+		do
+				-- Inheritance relation
+			-- TODO
+
+				-- Creation routines
+			process_creation_routines (a_class)
+
+				-- Normal features
+			process_features (a_class)
+		end
+
+	process_feature (a_feature: !FEATURE_I)
+			-- Generate code for `a_feature'.
+		do
+			put_comment_line ("Feature " + a_feature.feature_name + " from class " + a_feature.written_class.name_in_upper)
+			put_comment_line ("--------------------------------------")
+			put_new_line
+
+			if a_feature.is_attribute then
+					-- Generate field name, function and axiom
+				attribute_writer.write_attribute (a_feature)
+			elseif a_feature.is_constant then
+					-- Generate function and axiom
+				constant_writer.write_constant (a_feature)
+			else
+				if a_feature.type.is_void then
+						-- It's a query, so generate functional representation
+					-- TODO
+				end
+
+					-- Generate signature
+				signature_writer.write_feature_signature (a_feature)
+
+					-- Generate implementation
+				-- TODO: make this check look nicer
+				if verify_value_in_indexing (a_feature.written_class.ast.feature_with_name (a_feature.feature_name_id).indexes) then
+					implementation_writer.write_feature_implementation (a_feature)
+				else
+					put_comment_line ("Implementation ignored due to indexing clause")
+				end
+			end
+			put_new_line
+
+			feature_list.mark_feature_generated (a_feature)
+		ensure
+			feature_not_needed: not feature_list.features_needed.has (a_feature)
+			feature_generated: feature_list.features_generated.has (a_feature)
+		end
+
+	process_creation_routine (a_feature: !FEATURE_I)
+			-- Generate code for creation routine `a_feature'.
+		do
+			put_comment_line ("Creation routine " + a_feature.feature_name + " from class " + a_feature.written_class.name_in_upper)
+			put_comment_line ("--------------------------------------")
+			put_new_line
+
+				-- Generate signature
+			signature_writer.write_creation_routine_signature (a_feature)
+			put_new_line
+
+			feature_list.mark_creation_routine_as_generated (a_feature)
+		ensure
+			feature_not_needed: not feature_list.creation_routines_needed.has (a_feature)
+			feature_generated: feature_list.creation_routines_generated.has (a_feature)
+		end
+
+feature {NONE} -- Implementation
+
+	attribute_writer: !EP_ATTRIBUTE_WRITER
+			-- Writer to produce code for attributes
+
+	constant_writer: !EP_CONSTANT_WRITER
+			-- Writer to procude code for constants
+
+	signature_writer: !EP_SIGNATURE_WRITER
+			-- Writer to procduce feature signatures
+
+	implementation_writer: !EP_IMPLEMENTATION_WRITER
+			-- Writer to procduce feature implementations
+
+	process_creation_routines (a_class: !CLASS_C)
+			-- Process creation routines of class `a_class'.
+		local
+			l_creator_name: STRING
+			l_feature: FEATURE_I
+			l_attached_feature: !FEATURE_I
+		do
+			from
+				a_class.creators.start
+			until
+				a_class.creators.after
+			loop
+				l_creator_name := a_class.creators.key_for_iteration
+
+				l_feature := a_class.feature_named (l_creator_name)
+				l_attached_feature ?= l_feature
+				check l_feature /= Void end
+
+				process_creation_routine (l_attached_feature)
+
+				a_class.creators.forth
+			end
+		end
+
+	process_features (a_class: !CLASS_C)
+			-- Process features of class `a_class'.
+		local
+			l_feature: FEATURE_I
+			l_attached_feature: !FEATURE_I
+		do
+			from
+				a_class.feature_table.start
+			until
+				a_class.feature_table.after
+			loop
+				l_feature := a_class.feature_table.item_for_iteration
+				l_attached_feature ?= l_feature
+				check l_feature /= Void end
+
+					-- Only write features which are written in that class
+				if l_feature.written_in = a_class.class_id then
+					process_feature (l_attached_feature)
+				else
+					-- commented out as this gives to much unnecessary output
+					--put_comment_line ("ignored " + l_feature.feature_name)
+				end
+
+				a_class.feature_table.forth
+			end
+		end
+
+end
