ballet/63/Src/eve_proofs/eve_proofs.e
@@ -1,0 +1,229 @@
+indexing
+	description:
+		"[
+			Interface to use the verification system.
+		]"
+	date: "$Date$"
+	revision: "$Revision$"
+
+class EVE_PROOFS
+
+inherit {NONE}
+
+	SHARED_EP_ENVIRONMENT
+		export {NONE} all end
+
+	EB_SHARED_MANAGERS
+		export {NONE} all end
+
+	EV_SHARED_APPLICATION
+		export {NONE} all end
+
+create
+	make
+
+feature {NONE} -- Initialization
+
+	make is
+			-- Initialize object.
+		do
+			if {PLATFORM}.is_windows then
+				create verifier.make
+--				create {BOOGIE_WINDOWS_EXEC}verifier.make
+			else
+--				add_error (create {BPL_ERROR}.make("unsupported system for Ballet"))
+			end
+			create boogie_generator.make
+			create {LINKED_LIST [!CLASS_C]} classes_to_verify.make
+			is_file_per_class_generated := False
+		ensure
+			supporting_windows: {PLATFORM}.is_windows implies is_ready
+		end
+
+feature -- Access
+
+	classes_to_verify: !LIST [!CLASS_C]
+			-- Classes which will be verified
+
+feature -- Status report
+
+	is_ready: BOOLEAN
+			-- Is Ballet ready for verification?
+		do
+			Result := verifier /= Void
+		end
+
+	is_file_per_class_generated: BOOLEAN
+			-- Is a single file generated per verified class?
+
+feature -- Element change
+
+	add_class_to_verify (a_class: !CLASS_C)
+			-- Add `a_class' to `classes_to_verify'.
+		require
+			a_class_not_yet_added: not classes_to_verify.has (a_class)
+			a_class_is_eiffel_class: a_class.is_eiffel_class_c
+		do
+			classes_to_verify.extend (a_class)
+		ensure
+			a_class_added: classes_to_verify.has (a_class)
+		end
+
+feature -- Basic operations
+
+	reset
+			-- Reset the classes and feature.
+		do
+			classes_to_verify.wipe_out
+		ensure
+			no_classes_to_verify: classes_to_verify.is_empty
+		end
+
+	execute_verification
+			-- Execute verification on added classes.
+		require
+			class_added: not classes_to_verify.is_empty
+			ready: is_ready
+		local
+			l_current_class: !CLASS_C
+		do
+			output_manager.clear
+			show_messages ("Ballet started", "Ballet started")
+
+				-- Set up environment
+			set_up_environment
+
+				-- Generate Boogie code for classes
+			show_messages ("Generating Boogie code for:", "Generating Boogie code")
+			from
+				classes_to_verify.start
+			until
+				classes_to_verify.after
+			loop
+				l_current_class := classes_to_verify.item
+
+					-- Print byte nodes of class (for debugging)
+				print_byte_nodes (l_current_class)
+
+					-- Generate Boogie code of class
+					-- First check if class is ignored due to an indexing clause
+				if verify_value_in_indexing (l_current_class.ast.internal_top_indexes) then
+					show_messages (" - Class " + l_current_class.name_in_upper, "Generating Boogie code: " + l_current_class.name_in_upper)
+					generate_boogie_code (l_current_class)
+				else
+					show_messages (" - Class " + l_current_class.name_in_upper + " (ignored due to indexing clause)", "Generating Boogie code")
+				end
+
+				classes_to_verify.forth
+			variant
+				classes_to_verify.count - classes_to_verify.index + 1
+			end
+
+				-- Generate Boogie code for referenced features
+			show_messages(" - Referenced features", "Generating Boogie code: Referenced features")
+			generate_code_for_referenced_features
+
+				-- Start Boogie
+			show_messages("Starting verifier", "Running verifier")
+			verifier.verify
+
+				-- React on errors
+			-- TODO
+		end
+
+feature {NONE} -- Implementation
+
+	verifier: EP_VERIFIER
+			-- Verifier used to run Boogie
+
+	boogie_generator: EP_GENERATOR
+			-- Generator used to generate Boogie code
+
+	show_messages (l_output_line, l_status_bar: STRING)
+			-- Show `l_output_line' in output window and `l_status_bar' in status bar.
+		do
+			output_manager.add_string (l_output_line)
+			output_manager.add_new_line
+			output_manager.end_processing
+			window_manager.display_message (l_status_bar)
+			ev_application.process_events
+		end
+
+	set_up_environment
+			-- Set up environment for a new verification session.
+		do
+			feature_list.reset
+			verifier.add_file_content (inclusion_file_name)
+		end
+
+	print_byte_nodes (a_class: !CLASS_C)
+			-- Print byte node tree for debugging.
+		do
+			-- TODO
+		end
+
+	generate_boogie_code (a_class: !CLASS_C)
+			-- Generate Boogie code for `a_class'.
+		local
+			l_output_stream: KL_STRING_OUTPUT_STREAM
+			l_content, l_name: !STRING
+		do
+			create l_output_stream.make_empty
+			environment.set_output_buffer (l_output_stream)
+
+			boogie_generator.process_class (a_class)
+
+			check l_output_stream.string /= Void and a_class.name_in_upper /= Void end
+			l_content ?= l_output_stream.string
+			l_name ?= "Class: " + a_class.name_in_upper
+			verifier.add_string_content (l_content, l_name)
+		end
+
+	generate_code_for_referenced_features
+			-- Generate Boogie code for all referenced features.
+		local
+			l_list: !LIST [!FEATURE_I]
+			l_output_stream: KL_STRING_OUTPUT_STREAM
+			l_content: !STRING
+		do
+			create l_output_stream.make_empty
+			environment.set_output_buffer (l_output_stream)
+
+				-- Generate code for creation routines
+			from
+				l_list := feature_list.creation_routines_needed
+			until
+				l_list.is_empty
+			loop
+				boogie_generator.process_creation_routine (l_list.first)
+			end
+
+				-- Generate code for normal features
+			from
+				l_list := feature_list.features_needed
+			until
+				l_list.is_empty
+			loop
+				boogie_generator.process_feature (l_list.first)
+			end
+
+			l_content ?= l_output_stream.string
+			verifier.add_string_content (l_content, "Referenced features")
+		end
+
+
+-- TODO: move file someplace else
+	inclusion_file_name: !STRING is
+			-- Name of the file to include for the background theory
+		local
+			ee: EXECUTION_ENVIRONMENT
+		once
+			create ee
+			Result ?= ee.get("EIFFEL_SRC") + "/ballet/background_theory.bpl"
+		end
+
+
+
+anchor: SHARED_EP_OUTPUT_BUFFER
+
+end
