ballet/63/Src/eve_proofs/shared_ep_environment.e
@@ -1,0 +1,95 @@
+indexing
+	description: "Shared access to an EP_ENVIRONMENT"
+	author: ""
+	date: "$Date$"
+	revision: "$Revision$"
+
+class SHARED_EP_ENVIRONMENT
+
+feature -- Access
+
+	environment: EP_ENVIRONMENT
+			-- Shared Eve Proofs environement
+		once
+			create Result.make
+		end
+
+	feature_list: !EP_FEATURE_LIST
+		once
+			create Result.make
+		end
+
+	name_generator: !EP_DEFAULT_NAMES
+			-- Shared name generator
+		once
+			create Result
+		end
+
+	type_mapper: !EP_TYPE_MAPPER
+			-- Shared type mapper
+		once
+			create Result
+		end
+
+feature -- Convenience
+
+-- TODO: move to its own class?
+-- TODO: add 'indent' 'unindent' features
+
+	verify_value_in_indexing (a_indexing_clause: INDEXING_CLAUSE_AS): BOOLEAN
+			-- Value of the first indexing tag `Verify'
+			-- If the tag is not set, it will default to true.
+		local
+			l_index: INDEX_AS
+			l_bool: BOOL_AS
+			l_found: BOOLEAN
+		do
+			Result := True
+			if a_indexing_clause /= Void then
+				from
+					a_indexing_clause.start
+				until
+					a_indexing_clause.after or l_found
+				loop
+					l_index := a_indexing_clause.item
+						-- TODO: extract string literal
+					if l_index.tag.name.as_lower.is_equal ("verify") then
+						l_found := True
+						l_bool ?= l_index.index_list.first
+						if l_bool /= Void then
+							Result := l_bool.value
+						end
+					end
+					a_indexing_clause.forth
+				end
+			end
+		end
+
+	put (a_string: STRING)
+			-- Put `a_string' to output buffer.
+		do
+			environment.output_buffer.put_string (a_string)
+		end
+
+	put_line (a_line: STRING)
+			-- Put `a_line' to output buffer and append a new line.
+		do
+			environment.output_buffer.put_string (a_line)
+			environment.output_buffer.put_new_line
+		end
+
+	put_comment_line (a_line: STRING)
+			-- Put `a_line' to output buffer as a comment and append a new line.
+		do
+			environment.output_buffer.put_string ("// ")
+			environment.output_buffer.put_string (a_line)
+			environment.output_buffer.put_new_line
+		end
+
+	put_new_line
+			-- Put a new line to output buffer.
+		do
+			environment.output_buffer.put_new_line
+		end
+
+end
