ballet/63/Src/eve_proofs/writer/ep_constant_writer.e
@@ -1,0 +1,96 @@
+indexing
+	description:
+		"[
+			Boogie code writer for attributes.
+		]"
+	date: "$Date$"
+	revision: "$Revision$"
+
+class EP_CONSTANT_WRITER
+
+inherit {NONE}
+
+	SHARED_EP_ENVIRONMENT
+		export {NONE} all end
+
+feature -- Basic operations
+
+	write_constant (a_feature: !FEATURE_I)
+			-- Write Boogie code for `a_feature'.
+		require
+			is_constant: a_feature.is_constant
+		local
+			l_functional_name, l_type, l_value: STRING
+			l_constant: CONSTANT_I
+		do
+			l_constant ?= a_feature
+			check l_constant /= Void end
+
+			l_functional_name := name_generator.functional_feature_name (a_feature)
+			l_type := type_mapper.boogie_type_for_type (a_feature.type)
+
+			put_comment_line ("Functional represenation of constant")
+			put_line ("function " + l_functional_name + "(heap: [ref, <x>name]x, current: ref) returns (" + l_type + ";")
+			put_new_line
+
+			if l_constant.value.is_boolean then
+				l_value := boolean_value (l_constant.value)
+			elseif l_constant.value.is_integer then
+				l_value := integer_value (l_constant.value)
+			elseif l_constant.value.is_character then
+				l_value := character_value (l_constant.value)
+			else
+				-- TODO: add error
+			end
+
+			if l_value = Void then
+				put_comment_line ("Unsupported type, no axiom generated")
+			else
+				put_comment_line ("Axiomatic mapping of function to constant value")
+				put_line ("axiom (forall heap: [ref, <x>name]x, current: ref ::")
+				put_line ("            { " + l_functional_name + "(heap, current) } // Trigger");
+				put_line ("        IsHeap(heap) ==> (" + l_functional_name + "(heap, current) == " + l_value + "));")
+				put_new_line
+			end
+		end
+
+feature {NONE} -- Implementation
+
+	boolean_value (a_value: VALUE_I): STRING
+			-- Value of `a_value' for Boogie
+		require
+			a_value.is_boolean
+		local
+			l_bool: BOOL_VALUE_I
+		do
+			l_bool ?= a_value
+			if l_bool.boolean_value then
+				Result := "true"
+			else
+				Result := "false"
+			end
+		end
+
+	integer_value (a_value: VALUE_I): STRING
+			-- Value of `a_value' for Boogie
+		require
+			a_value.is_integer
+		local
+			l_int: INTEGER_CONSTANT
+		do
+			l_int ?= a_value
+			Result := l_int.integer_32_value.out
+		end
+
+	character_value (a_value: VALUE_I): STRING
+			-- Value of `a_value' for Boogie
+		require
+			a_value.is_character
+		local
+			l_char: CHAR_VALUE_I
+		do
+			l_char ?= a_value
+			Result := l_char.character_value.code.out
+		end
+
+end
