ballet/63/Src/eve_proofs/writer/ep_expression_writer.e
@@ -1,0 +1,50 @@
+indexing
+	description:
+		"[
+			Boogie code writer to generate expressions
+		]"
+	date: "$Date$"
+	revision: "$Revision$"
+
+class EP_EXPRESSION_WRITER
+
+inherit
+
+	SHARED_EP_ENVIRONMENT
+		export {NONE} all end
+
+	EP_DEFAULT_NAMES
+		export {NONE} all end
+
+create
+	make
+
+feature {NONE} -- Initialization
+
+	make (a_mapper: !EP_NAME_MAPPER)
+			-- Initialize expression writer with `a_mapper'.
+		do
+			name_mapper := a_mapper
+		ensure
+			name_mapper_set: name_mapper = a_mapper
+		end
+
+feature -- Access
+
+	name_mapper: !EP_NAME_MAPPER
+			-- Name mapper used to create Boogie code names
+
+	old_handler: !EP_OLD_HANDLER
+			-- Handler for old expressions
+
+feature -- Element change
+
+	set_name_mapper (a_mapper: like name_mapper)
+			-- Set `name_mapper' to `a_name_mapper'.
+		do
+			name_mapper := a_mapper
+		ensure
+			name_mapper_set: name_mapper = a_mapper
+		end
+
+end
