ballet/63/Src/eve_proofs/writer/ep_function_writer.e
@@ -1,0 +1,19 @@
+indexing
+	description:
+		"[
+			Boogie code writer to generate functions
+		]"
+	date: "$Date$"
+	revision: "$Revision$"
+
+class EP_FUNCTION_WRITER
+
+inherit
+
+	SHARED_EP_ENVIRONMENT
+		export {NONE} all end
+
+	EP_DEFAULT_NAMES
+		export {NONE} all end
+
+end
