ballet/63/Src/eve_proofs/writer/ep_implementation_writer.e
@@ -1,0 +1,69 @@
+indexing
+	description:
+		"[
+			Boogie code writer to generate feature implementations
+		]"
+	date: "$Date$"
+	revision: "$Revision$"
+
+class EP_IMPLEMENTATION_WRITER
+
+inherit
+
+	SHARED_EP_ENVIRONMENT
+		export {NONE} all end
+
+	EP_DEFAULT_NAMES
+		export {NONE} all end
+
+create
+	make
+
+feature {NONE} -- Initialization
+
+	make
+			-- TODO
+		do
+
+		end
+
+feature -- Basic operations
+
+	write_feature_implementation (a_feature: !FEATURE_I)
+			-- Write Boogie code for implementation of `a_feature'.
+		local
+			l_procedure_name: STRING
+			i: INTEGER
+			l_argument_name: STRING
+			l_argument_type: TYPE_A
+		do
+			l_procedure_name := procedural_feature_name (a_feature)
+
+			put_comment_line ("Implementation")
+
+			-- TODO: code reuse with signature writer => inherit from signature writer?
+
+			put ("implementation " + l_procedure_name + "(Current: ref")
+			from
+				i := 1
+			until
+				i > a_feature.argument_count
+			loop
+				l_argument_name := a_feature.arguments.item_name (i)
+				l_argument_type := a_feature.arguments.i_th (i)
+				put (", " + l_argument_name + ": " + type_mapper.boogie_type_for_type (l_argument_type))
+				i := i + 1
+			end
+			put (")")
+			if not a_feature.type.is_void then
+				put (" returns (Result: " + type_mapper.boogie_type_for_type (a_feature.type) + ")")
+			end
+			put (";%N")
+			put_line ("{")
+
+			-- TODO
+
+			put_line ("}")
+		end
+
+end
