ballet/63/Src/eve_proofs/writer/ep_name_mapper.e
@@ -1,0 +1,43 @@
+indexing
+	description:
+		"[
+			Name mapping for varibales
+		]"
+	date: "$Date$"
+	revision: "$Revision$"
+
+deferred class EP_NAME_MAPPER
+
+feature -- Access
+
+	heap_name: STRING
+			-- Name of heap in Boogie code
+		deferred
+		end
+
+	current_name (a_node: CURRENT_B): STRING
+			-- Name of current reference in Boogie code
+		deferred
+		end
+
+	result_name (a_node: RESULT_B): STRING
+			-- Name of result reference in Boogie code
+		deferred
+		end
+
+	argument_name (a_node: ARGUMENT_B): STRING
+			-- Name of argument in Boogie code
+		deferred
+		end
+
+	feature_name (a_node: FEATURE_B): STRING
+			-- Name of feature in Boogie code
+		deferred
+		end
+
+	local_name (a_node: LOCAL_B): STRING
+			-- Name of local in Boogie code
+		deferred
+		end
+
+end
