ballet/63/Src/eve_proofs/writer/ep_normal_name_mapper.e
@@ -1,0 +1,70 @@
+indexing
+	description:
+		"[
+			TODO
+		]"
+	date: "$Date$"
+	revision: "$Revision$"
+
+class EP_NORMAL_NAME_MAPPER
+
+inherit
+
+	EP_NAME_MAPPER
+
+	SHARED_EP_ENVIRONMENT
+		export {NONE} all end
+
+create
+	make
+
+feature {NONE} -- Initialization
+
+	make
+			-- TODO
+		do
+
+		end
+
+feature -- Access
+
+	current_feature: !FEATURE_I
+			-- Current feature where mapping is made
+
+	heap_name: STRING
+			-- Name of heap in Boogie code
+		do
+			Result := "Heap"
+		end
+
+	current_name (a_node: CURRENT_B): STRING
+			-- Name of current reference in Boogie code
+		do
+			Result := "Current"
+		end
+
+	result_name (a_node: RESULT_B): STRING
+			-- Name of result reference in Boogie code
+		do
+			Result := "Result"
+		end
+
+	argument_name (a_node: ARGUMENT_B): STRING
+			-- Name of argument in Boogie code
+		do
+			Result := name_generator.argument_name (current_feature.arguments.item_name (a_node.position))
+		end
+
+	feature_name (a_node: FEATURE_B): STRING
+			-- Name of feature in Boogie code
+		do
+
+		end
+
+	local_name (a_node: LOCAL_B): STRING
+			-- Name of local in Boogie code
+		do
+
+		end
+
+end
