ballet/63/Src/eve_proofs/writer/ep_old_handler.e
@@ -1,0 +1,8 @@
+indexing
+	description: "Summary description for {EP_OLD_HANDLER}."
+	date: "$Date$"
+	revision: "$Revision$"
+
+deferred class EP_OLD_HANDLER
+
+end
