ballet/63/Src/eve_proofs/writer/ep_signature_writer.e
@@ -1,0 +1,94 @@
+indexing
+	description:
+		"[
+			Boogie code writer to generate feature signatures
+		]"
+	date: "$Date$"
+	revision: "$Revision$"
+
+class EP_SIGNATURE_WRITER
+
+inherit
+
+	SHARED_EP_ENVIRONMENT
+		export {NONE} all end
+
+create
+	make
+
+feature {NONE} -- Initialization
+
+	make
+			-- TODO
+		do
+
+		end
+
+feature -- Basic operations
+
+	write_feature_signature (a_feature: !FEATURE_I)
+			-- Write Boogie code signature of `a_feature'.
+		local
+			l_procedure_name: STRING
+			i: INTEGER
+			l_argument_name: STRING
+			l_argument_type: TYPE_A
+		do
+			l_procedure_name := name_generator.procedural_feature_name (a_feature)
+
+			put_comment_line ("Signature")
+
+			put ("procedure " + l_procedure_name + "(")
+			if a_feature.argument_count = 0 then
+				put ("Current: ref where Current != null && Heap[Current, $allocated]")
+			else
+				put ("%N")
+				put ("            Current: ref where Current != null && Heap[Current, $allocated]")
+
+				from
+					i := 1
+				until
+					i > a_feature.argument_count
+				loop
+					l_argument_name :=  name_generator.argument_name (a_feature.arguments.item_name (i))
+					l_argument_type := a_feature.arguments.i_th (i)
+
+					put (",%N")
+					put ("            " + l_argument_name + ": " + type_mapper.boogie_type_for_type (l_argument_type))
+					if not l_argument_type.is_expanded then
+						if l_argument_type.is_attached then
+							put (" where " + l_argument_name + " != null && Heap[" + l_argument_name + ", $allocated]")
+						else
+							put (" where " + l_argument_name + " != null ==> Heap[" + l_argument_name + ", $allocated]")
+						end
+					end
+
+					i := i + 1
+				end
+				put ("%N        ")
+			end
+
+			put (")")
+			if not a_feature.type.is_void then
+				put (" returns (Result: " + type_mapper.boogie_type_for_type (a_feature.type) + ")")
+			end
+			put (";%N")
+
+			-- TODO: generate preconditions
+
+			put_line ("    modifies Heap;")
+
+			-- TODO: generate postconditions
+
+			-- TODO: generate invariants
+
+			put_new_line
+		end
+
+	write_creation_routine_signature (a_feature: !FEATURE_I)
+			-- Write Boogie code signature of `a_feature' as a creation routine.
+		do
+			-- TODO
+		end
+
+end
