ballet/63/Src/eve_proofs/writer/ep_visitor.e
@@ -1,0 +1,602 @@
+indexing
+	description:
+		"[
+			TODO
+		]"
+	date: "$Date$"
+	revision: "$Revision$"
+
+deferred class EP_VISITOR
+
+inherit
+
+	BYTE_NODE_VISITOR
+
+feature {BYTE_NODE} -- Visitors
+
+	process_access_expr_b (a_node: ACCESS_EXPR_B) is
+			-- Process `a_node'.
+		do
+			safe_process (a_node.expr)
+		end
+
+	process_address_b (a_node: ADDRESS_B) is
+			-- Process `a_node'.
+		do
+			-- No Subnode
+		end
+
+	process_argument_b (a_node: ARGUMENT_B) is
+			-- Process `a_node'.
+		do
+			-- No Subnode
+		end
+
+	process_array_const_b (a_node: ARRAY_CONST_B) is
+			-- Process `a_node'.
+		do
+			safe_process (a_node.expressions)
+		end
+
+	process_assert_b (a_node: ASSERT_B) is
+			-- Process `a_node'.
+		do
+			safe_process (a_node.expr)
+		end
+
+	process_assign_b (a_node: ASSIGN_B) is
+			-- Process `a_node'.
+		do
+			safe_process (a_node.target)
+			safe_process (a_node.source)
+		end
+
+	process_attribute_b (a_node: ATTRIBUTE_B) is
+			-- Process `a_node'.
+		do
+			-- No Subnode
+		end
+
+	process_bin_and_b (a_node: BIN_AND_B) is
+			-- Process `a_node'.
+		do
+			safe_process (a_node.left)
+			safe_process (a_node.right)
+		end
+
+	process_bin_and_then_b (a_node: B_AND_THEN_B) is
+			-- Process `a_node'.
+		do
+			safe_process (a_node.left)
+			safe_process (a_node.right)
+		end
+
+	process_bin_div_b (a_node: BIN_DIV_B) is
+			-- Process `a_node'.
+		do
+			safe_process (a_node.left)
+			safe_process (a_node.right)
+		end
+
+	process_bin_eq_b (a_node: BIN_EQ_B) is
+			-- Process `a_node'.
+		do
+			safe_process (a_node.left)
+			safe_process (a_node.right)
+		end
+
+	process_bin_free_b (a_node: BIN_FREE_B) is
+			-- Process `a_node'.
+		do
+			safe_process (a_node.left)
+			safe_process (a_node.right)
+		end
+
+	process_bin_ge_b (a_node: BIN_GE_B) is
+			-- Process `a_node'.
+		do
+			safe_process (a_node.left)
+			safe_process (a_node.right)
+		end
+
+	process_bin_gt_b (a_node: BIN_GT_B) is
+			-- Process `a_node'.
+		do
+			safe_process (a_node.left)
+			safe_process (a_node.right)
+		end
+
+	process_bin_implies_b (a_node: B_IMPLIES_B) is
+			-- Process `a_node'.
+		do
+			safe_process (a_node.left)
+			safe_process (a_node.right)
+		end
+
+	process_bin_le_b (a_node: BIN_LE_B) is
+			-- Process `a_node'.
+		do
+			safe_process (a_node.left)
+			safe_process (a_node.right)
+		end
+
+	process_bin_lt_b (a_node: BIN_LT_B) is
+			-- Process `a_node'.
+		do
+			safe_process (a_node.left)
+			safe_process (a_node.right)
+		end
+
+	process_bin_minus_b (a_node: BIN_MINUS_B) is
+			-- Process `a_node'.
+		do
+			safe_process (a_node.left)
+			safe_process (a_node.right)
+		end
+
+	process_bin_mod_b (a_node: BIN_MOD_B) is
+			-- Process `a_node'.
+		do
+			safe_process (a_node.left)
+			safe_process (a_node.right)
+		end
+
+	process_bin_ne_b (a_node: BIN_NE_B) is
+			-- Process `a_node'.
+		do
+			safe_process (a_node.left)
+			safe_process (a_node.right)
+		end
+
+	process_bin_or_b (a_node: BIN_OR_B) is
+			-- Process `a_node'.
+		do
+			safe_process (a_node.left)
+			safe_process (a_node.right)
+		end
+
+	process_bin_or_else_b (a_node: B_OR_ELSE_B) is
+			-- Process `a_node'.
+		do
+			safe_process (a_node.left)
+			safe_process (a_node.right)
+		end
+
+	process_bin_plus_b (a_node: BIN_PLUS_B) is
+			-- Process `a_node'.
+		do
+			safe_process (a_node.left)
+			safe_process (a_node.right)
+		end
+
+	process_bin_power_b (a_node: BIN_POWER_B) is
+			-- Process `a_node'.
+		do
+			safe_process (a_node.left)
+			safe_process (a_node.right)
+		end
+
+	process_bin_slash_b (a_node: BIN_SLASH_B) is
+			-- Process `a_node'.
+		do
+			safe_process (a_node.left)
+			safe_process (a_node.right)
+		end
+
+	process_bin_star_b (a_node: BIN_STAR_B) is
+			-- Process `a_node'.
+		do
+			safe_process (a_node.left)
+			safe_process (a_node.right)
+		end
+
+	process_bin_xor_b (a_node: BIN_XOR_B) is
+			-- Process `a_node'.
+		do
+			safe_process (a_node.left)
+			safe_process (a_node.right)
+		end
+
+	process_bit_const_b (a_node: BIT_CONST_B) is
+			-- Process `a_node'.
+		do
+			-- No subnode
+		end
+
+	process_bool_const_b (a_node: BOOL_CONST_B) is
+			-- Process `a_node'.
+		do
+			-- No Subnode
+		end
+
+	process_byte_list (a_node: BYTE_LIST [BYTE_NODE]) is
+			-- Process `a_node'.
+		local
+			i: INTEGER
+			c: INTEGER
+		do
+			from
+				i := 1
+				c := a_node.count
+			until
+				i > c
+			loop
+				safe_process (a_node.i_th (i))
+				i := i + 1
+			end
+		end
+
+	process_case_b (a_node: CASE_B) is
+			-- Process `a_node'.
+		do
+			safe_process (a_node.compound)
+			safe_process (a_node.interval)
+		end
+
+	process_char_const_b (a_node: CHAR_CONST_B) is
+			-- Process `a_node'.
+		do
+			-- No Subnode
+		end
+
+	process_char_val_b (a_node: CHAR_VAL_B) is
+			-- Process `a_node'.
+		do
+			-- No Subnode
+		end
+
+	process_check_b (a_node: CHECK_B) is
+			-- Process `a_node'.
+		do
+			safe_process (a_node.check_list)
+		end
+
+	process_constant_b (a_node: CONSTANT_B) is
+			-- Process `a_node'.
+		do
+			safe_process (a_node.access)
+		end
+
+	process_creation_expr_b (a_node: CREATION_EXPR_B) is
+			-- Process `a_node'.
+		do
+			safe_process (a_node.call)
+		end
+
+	process_current_b (a_node: CURRENT_B) is
+			-- Process `a_node'.
+		do
+			-- No subnode
+		end
+
+	process_custom_attribute_b (a_node: CUSTOM_ATTRIBUTE_B) is
+			-- Process `a_node'.
+		do
+			safe_process (a_node.creation_expr)
+			-- TODO: Names arguments
+		end
+
+	process_debug_b (a_node: DEBUG_B) is
+			-- Process `a_node'.
+		do
+			safe_process (a_node.compound)
+		end
+
+	process_elsif_b (a_node: ELSIF_B) is
+			-- Process `a_node'.
+		do
+			safe_process (a_node.expr)
+		end
+
+	process_expr_address_b (a_node: EXPR_ADDRESS_B) is
+			-- Process `a_node'.
+		do
+			safe_process (a_node.expr)
+		end
+
+	process_external_b (a_node: EXTERNAL_B) is
+			-- Process `a_node'.
+		do
+			safe_process (a_node.parameters)
+		end
+
+	process_feature_b (a_node: FEATURE_B) is
+			-- Process `a_node'.
+		do
+			safe_process (a_node.parameters)
+		end
+
+	process_frame_b (a_node: FRAME_B) is
+			-- Process `a_node'.
+		do
+			safe_process (a_node.expr)
+		end
+
+	process_agent_call_b (a_node: AGENT_CALL_B) is
+		do
+			safe_process (a_node.parameters)
+		end
+
+	process_formal_conversion_b (a_node: FORMAL_CONVERSION_B) is
+			-- Process `a_node'.
+		do
+			safe_process (a_node.expr)
+		end
+
+	process_hector_b (a_node: HECTOR_B) is
+			-- Process `a_node'.
+		do
+			safe_process (a_node.access)
+			safe_process (a_node.expr)
+		end
+
+	process_if_b (a_node: IF_B) is
+			-- Process `a_node'.
+		do
+			safe_process (a_node.condition)
+			safe_process (a_node.compound)
+			safe_process (a_node.elsif_list)
+			safe_process (a_node.else_part)
+		end
+
+	process_inspect_b (a_node: INSPECT_B) is
+			-- Process `a_node'.
+		do
+			safe_process (a_node.switch)
+			safe_process (a_node.case_list)
+			safe_process (a_node.else_part)
+		end
+
+	process_instr_call_b (a_node: INSTR_CALL_B) is
+			-- Process `a_node'.
+		do
+			safe_process (a_node.call)
+		end
+
+	process_instr_list_b (a_node: INSTR_LIST_B) is
+			-- Process `a_node'.
+		do
+			safe_process (a_node.compound)
+		end
+
+	process_int64_val_b (a_node: INT64_VAL_B) is
+			-- Process `a_node'.
+		do
+			-- No Subnode
+		end
+
+	process_int_val_b (a_node: INT_VAL_B) is
+			-- Process `a_node'.
+		do
+			-- No Subnode
+		end
+
+	process_integer_constant (a_node: INTEGER_CONSTANT) is
+			-- Process `a_node'.
+		do
+			-- No Subnode
+		end
+
+	process_inv_assert_b (a_node: INV_ASSERT_B) is
+			-- Process `a_node'.
+		do
+			safe_process (a_node.expr)
+		end
+
+	process_invariant_b (a_node: INVARIANT_B) is
+			-- Process `a_node'.
+		do
+			safe_process (a_node.byte_list)
+		end
+
+	process_local_b (a_node: LOCAL_B) is
+			-- Process `a_node'.
+		do
+			-- No Subnode
+		end
+
+	process_loop_b (a_node: LOOP_B) is
+			-- Process `a_node'.
+		do
+			safe_process (a_node.from_part)
+			safe_process (a_node.stop)
+			safe_process (a_node.invariant_part)
+			safe_process (a_node.variant_part)
+			safe_process (a_node.compound)
+		end
+
+	process_nat64_val_b (a_node: NAT64_VAL_B) is
+			-- Process `a_node'.
+		do
+			-- No Subnode
+		end
+
+	process_nat_val_b (a_node: NAT_VAL_B) is
+			-- Process `a_node'.
+		do
+			-- No Subnode
+		end
+
+	process_nested_b (a_node: NESTED_B) is
+			-- Process `a_node'.
+		do
+			safe_process (a_node.target)
+			safe_process (a_node.message)
+		end
+
+	process_once_string_b (a_node: ONCE_STRING_B) is
+			-- Process `a_node'.
+		do
+			-- No Subnode
+		end
+
+	process_operand_b (a_node: OPERAND_B) is
+			-- Process `a_node'.
+		do
+			-- No Subnode
+		end
+
+	process_parameter_b (a_node: PARAMETER_B) is
+			-- Process `a_node'.
+		do
+			safe_process (a_node.expression)
+		end
+
+	process_paran_b (a_node: PARAN_B) is
+			-- Process `a_node'.
+		do
+			safe_process (a_node.expr)
+		end
+
+	process_real_const_b (a_node: REAL_CONST_B) is
+			-- Process `a_node'.
+		do
+			-- No Subnode
+		end
+
+	process_require_b (a_node: REQUIRE_B) is
+			-- Process `a_node'.
+		do
+			safe_process (a_node.expr)
+		end
+
+	process_result_b (a_node: RESULT_B) is
+			-- Process `a_node'.
+		do
+			-- No Subnode
+		end
+
+	process_retry_b (a_node: RETRY_B) is
+			-- Process `a_node'.
+		do
+			-- No Subnode
+		end
+
+	process_reverse_b (a_node: REVERSE_B) is
+			-- Process `a_node'.
+		do
+			safe_process (a_node.target)
+			safe_process (a_node.source)
+		end
+
+	process_routine_creation_b (a_node: ROUTINE_CREATION_B) is
+			-- Process `a_node'.
+		do
+			-- TODO: Do not understand this
+		end
+
+	process_string_b (a_node: STRING_B) is
+			-- Process `a_node'.
+		do
+			-- No Subnode
+		end
+
+	process_strip_b (a_node: STRIP_B) is
+			-- Process `a_node'.
+		do
+			-- No Subnode
+		end
+
+	process_tuple_access_b (a_node: TUPLE_ACCESS_B) is
+			-- Process `a_node'.
+		do
+			safe_process (a_node.source)
+		end
+
+	process_tuple_const_b (a_node: TUPLE_CONST_B) is
+			-- Process `a_node'.
+		do
+			safe_process (a_node.expressions)
+		end
+
+	process_type_expr_b (a_node: TYPE_EXPR_B) is
+			-- Process `a_node'.
+		do
+			-- No subnode
+		end
+
+	process_typed_interval_b (a_node: TYPED_INTERVAL_B [INTERVAL_VAL_B]) is
+			-- Process `a_node'.
+		do
+			safe_process (a_node.lower)
+			safe_process (a_node.upper)
+		end
+
+	process_un_free_b (a_node: UN_FREE_B) is
+			-- Process `a_node'.
+		do
+			safe_process (a_node.access)
+			safe_process (a_node.expr)
+		end
+
+	process_un_minus_b (a_node: UN_MINUS_B) is
+			-- Process `a_node'.
+		do
+			safe_process (a_node.access)
+			safe_process (a_node.expr)
+		end
+
+	process_un_not_b (a_node: UN_NOT_B) is
+			-- Process `a_node'.
+		do
+			safe_process (a_node.access)
+			safe_process (a_node.expr)
+		end
+
+	process_un_old_b (a_node: UN_OLD_B) is
+			-- Process `a_node'.
+		do
+			safe_process (a_node.access)
+			safe_process (a_node.expr)
+		end
+
+	process_un_plus_b (a_node: UN_PLUS_B) is
+			-- Process `a_node'.
+		do
+			safe_process (a_node.access)
+			safe_process (a_node.expr)
+		end
+
+	process_variant_b (a_node: VARIANT_B) is
+			-- Process `a_node'.
+		do
+			safe_process (a_node.expr)
+		end
+
+	process_void_b (a_node: VOID_B) is
+			-- Process `a_node'.
+		do
+			-- No subnode
+		end
+
+	process_object_test_b (a_node: OBJECT_TEST_B) is
+			-- Process `a_node'.
+		do
+			-- TODO
+		end
+
+	process_object_test_local_b (a_node: OBJECT_TEST_LOCAL_B) is
+			-- Process `a_node'.
+		do
+			-- TODO
+		end
+
+	process_bin_tilde_b (a_node: BIN_TILDE_B) is
+			-- Process `a_node'.
+		do
+			-- TODO
+		end
+
+	process_bin_not_tilde_b (a_node: BIN_NOT_TILDE_B) is
+			-- Process `a_node'.
+		do
+			-- TODO
+		end
+
+	process_std_byte_code (a_node: STD_BYTE_CODE) is
+			-- Process `a_node'.
+		do
+			-- TODO
+		end
+
+end
